---
created: 2024-09-09T12:17
updated: 2024-09-09T17:01
---
N1 
$$
\begin{array}\
\begin{pmatrix}
1 & 2 & 3
\end{pmatrix}
\cdot\begin{pmatrix}
-1 & -2 & -3 \\
1 & 0 & 0
\end{pmatrix}^{T}+\begin{pmatrix}
4 & 9
\end{pmatrix} \\
= \begin{pmatrix}
1 & 2 & 3
\end{pmatrix}
\cdot\begin{pmatrix}
-1 & 1 \\
-2 & 0 \\
-3 & 0
\end{pmatrix}+\begin{pmatrix}
4 & 9
\end{pmatrix} \\
= \begin{pmatrix}
-14 & 1
\end{pmatrix}+\begin{pmatrix}
4 & 9
\end{pmatrix}=\begin{pmatrix}
-10 & 10
\end{pmatrix}
\end{array}
$$
N2
1. 
$$
\begin{array}\
\begin{pmatrix}
3 & -4 & 5 \\
2 & -3 & 1 \\
3 & -5 & -1
\end{pmatrix} \cdot \begin{pmatrix}
3  & 29 \\
2 & 18  \\
0 & -3
\end{pmatrix} = \begin{pmatrix}
1 & 0 \\
0  & 1 \\
-1 & 0
\end{pmatrix}
\end{array}
$$
2. $$
\begin{array}\
\begin{pmatrix}
\cos \alpha & -\sin\alpha \\
\sin\alpha & \cos\alpha
\end{pmatrix} \cdot \begin{pmatrix}
\cos \beta & -\sin \beta \\
\sin\beta & \cos\beta
\end{pmatrix}  \\
= \begin{pmatrix}
\cos \alpha \cos\beta -\sin\alpha\sin \beta & -\cos \alpha \sin\beta -\sin\alpha\cos\beta \\
\sin\alpha\cos\beta +\cos\alpha\sin\beta & -\sin\alpha\sin\beta+\cos\alpha\cos\beta
\end{pmatrix} \\
= \begin{pmatrix}
\cos(\alpha+\beta) & -\sin(\alpha+\beta) \\
\sin(\alpha+\beta) & \cos(\alpha+\beta)
\end{pmatrix}
\end{array}
$$
3. $$
\begin{array}\
\begin{pmatrix}
0 & 1 & 0 & 0 \\
0 & 0 & 1 & 0 \\
0 & 0 & 0 & 1  \\
0 & 0 & 0 & 0 
\end{pmatrix}^{3}=\begin{pmatrix}
0 & 1 & 0 & 0 \\
0 & 0 & 1 & 0 \\
0 & 0 & 0 & 1  \\
0 & 0 & 0 & 0 
\end{pmatrix}^{2}\cdot\begin{pmatrix}
0 & 1 & 0 & 0 \\
0 & 0 & 1 & 0 \\
0 & 0 & 0 & 1  \\
0 & 0 & 0 & 0 
\end{pmatrix} \\
=\begin{pmatrix}
0 & 0 & 1 & 0 \\
0 & 0 & 0 & 1 \\
0 & 0 & 0 & 0  \\
0 & 0 & 0 & 0 
\end{pmatrix}\cdot\begin{pmatrix}
0 & 1 & 0 & 0 \\
0 & 0 & 1 & 0 \\
0 & 0 & 0 & 1  \\
0 & 0 & 0 & 0 
\end{pmatrix} =\begin{pmatrix}
0 & 0 & 0 & 1 \\
0 & 0 & 0 & 0 \\
0 & 0 & 0 & 0  \\
0 & 0 & 0 & 0 
\end{pmatrix}
\end{array}
$$
4. $$
\begin{array}\ \\
\begin{pmatrix}
\lambda_{1} & 0 & \dots & 0 \\
0 & \lambda_{2} & \dots & \dots \\
\dots & \dots & \dots & 0  \\
0 & \dots & 0 & \lambda_{n} 
\end{pmatrix}^{5}=\begin{pmatrix}
\lambda_{1}^{5} & 0 & \dots & 0 \\
0 & \lambda_{2}^{5} & \dots & \dots \\
\dots & \dots & \dots & 0  \\
0 & \dots & 0 & \lambda_{n}^{5}
\end{pmatrix}
\end{array}
$$
N3
$$
\begin{array}\
f(x)=x^{3}-3x+2 \\
A=\begin{pmatrix}
2 & 1 & 1 \\
1 & 2 & 1 \\
1 & 1 & 2
\end{pmatrix} \\ \\
f(A)=A^{3}-3A+2E \\ \\
f(A)=\begin{pmatrix}
2 & 1 & 1 \\
1 & 2 & 1 \\
1 & 1 & 2
\end{pmatrix}^{3}-3\cdot\begin{pmatrix}
2 & 1 & 1 \\
1 & 2 & 1 \\
1 & 1 & 2
\end{pmatrix}+2\cdot\begin{pmatrix}
1 & 0 & 0 \\
0 & 1 & 0 \\
0 & 0 & 1
\end{pmatrix} \\
= \begin{pmatrix}
22  & 21 & 21 \\
21 & 22 & 21 \\
21 & 21 & 22
\end{pmatrix}-\begin{pmatrix}
6 & 3 & 3 \\
3 & 6 & 3 \\
3 & 3 & 6
\end{pmatrix}+\begin{pmatrix}
2 & 0 & 0 \\
0 & 2 & 0 \\
0 & 0 & 2
\end{pmatrix} \\
=\begin{pmatrix}
18 & 18 & 18 \\
18 & 18 & 18 \\
18 & 18 & 18
\end{pmatrix}
\end{array}
$$
N4
$$
\begin{array}\
X=\begin{pmatrix}
a & b  \\
c & d
\end{pmatrix} \\
 \\
X^{2}-(a+d)X+(ad-bc)E \\
=\begin{pmatrix}
a & b  \\
c & d
\end{pmatrix}^{2}-(a+d)\begin{pmatrix}
a & b  \\
c & d
\end{pmatrix}+(ad-bc)\cdot\begin{pmatrix}
1 & 0 \\
0 & 1
\end{pmatrix} \\
=\begin{pmatrix}
a^{2}+bc & ab+bd \\
ac+dc & bc+d^2
\end{pmatrix}-\begin{pmatrix}
a^2+ad & ab+bd \\
ac+dc & ad+d^{2}
\end{pmatrix}+\begin{pmatrix}
ad-bc & 0 \\
0 & ad-bc
\end{pmatrix} \\
=\begin{pmatrix}
a^{2}+bc-a^{2}-ad+ad-bc & ab+bd-ab-bd \\
ac+dc-ac-dc & bc+d^{2}-ad-d^{2}+ad-bc
\end{pmatrix} \\
=\begin{pmatrix}
0 & 0 \\
0 & 0
\end{pmatrix}=\mathbb{O}
\end{array}
$$
N5
$$
\begin{array}\
AX=B; A=\begin{pmatrix}
1 & 3 \\
1 & 2
\end{pmatrix}; B=\begin{pmatrix}
1 & 1 \\
1 & 1
\end{pmatrix} \\
\text{пусть:}\;X=\begin{pmatrix}
a & b \\
c & d
\end{pmatrix} \\
B=\begin{pmatrix}
a+3c & b+3d \\
a+2c & b+2d
\end{pmatrix}=\begin{pmatrix}
1 & 1 \\
1 & 1
\end{pmatrix} \\ \\
\begin{cases}
a+3c=1 \\
a+2c=1 \\
b+3d=1 \\
b+2d=1
\end{cases}\Rightarrow\begin{cases}
a=1 \\
b=1 \\
c=0 \\
d=0
\end{cases} \\ \\
X=\begin{pmatrix}
1 & 1 \\
0 & 0
\end{pmatrix}
\end{array}
$$
N6
$$
\begin{array}\
AX=XA;\;  A=\begin{pmatrix}
0 & 1 \\
2 & 3
\end{pmatrix};\;  X=\begin{pmatrix}
a & b \\
c & d
\end{pmatrix}=\;? \\
AX=\begin{pmatrix}
c & d \\
2a+3c & 2b+3d
\end{pmatrix}=XA=\begin{pmatrix}
2b & a+3b \\
2d & c+3d
\end{pmatrix} \\
 \\
\Rightarrow\begin{cases}
c=2b \\
d=a+3b \\
2a+3c=2d \\
2b+3d=c+3d
\end{cases}\Rightarrow\begin{cases}
c=2b \\
d=a+3b \\
\end{cases} \\ \\
X=\begin{pmatrix}
a & b \\
2b & a+3b
\end{pmatrix}
\end{array}
$$
N7
$$
\begin{array}\
\begin{pmatrix}
17 & -6 \\
5 & -2
\end{pmatrix}=\begin{pmatrix}
2 & 3 \\
5 & 7
\end{pmatrix}\begin{pmatrix}
2 & 0 \\
0 & 3
\end{pmatrix}
\begin{pmatrix}
-7 & 3 \\
5 & -2
\end{pmatrix} \\
\begin{pmatrix}
-7 & 3 \\
5 & -2
\end{pmatrix}\begin{pmatrix}
2 & 3 \\
5 & 7
\end{pmatrix}=\begin{pmatrix}
0 & 0 \\
0 & 0
\end{pmatrix}=E \\
\begin{pmatrix}
17 & -6 \\
5 & -2
\end{pmatrix}^{5}=(\dots)(\dots)(\dots)\cdot(\dots)(\dots)(\dots)\cdot\; \dots\; \cdot(\dots)(\dots)(\dots) \\
=\begin{pmatrix}
2 & 3 \\
5 & 7
\end{pmatrix}\begin{pmatrix}
2 & 0 \\
0 & 3
\end{pmatrix}\cdot E \cdot\begin{pmatrix}
2 & 0 \\
0 & 3
\end{pmatrix}\cdot E\cdot \dots\;\cdot\begin{pmatrix}
2 & 0 \\
0 & 3
\end{pmatrix}\cdot\begin{pmatrix}
-7 & 3 \\
5 & -2
\end{pmatrix} \\
=\begin{pmatrix}
2 & 3 \\
5 & 7
\end{pmatrix}\begin{pmatrix}
2 & 0 \\
0 & 3
\end{pmatrix}^{5}
\begin{pmatrix}
-7 & 3 \\
5 & -2
\end{pmatrix} \\
=\begin{pmatrix}
2 & 3 \\
5 & 7
\end{pmatrix}\begin{pmatrix}
32 &  0 \\
0 & 243
\end{pmatrix}
\begin{pmatrix}
-7 & 3 \\
5 & -2
\end{pmatrix} \\
=\begin{pmatrix}
64 & 729\\
160 & 1701
\end{pmatrix}
\begin{pmatrix}
-7 & 3 \\
5 & -2
\end{pmatrix} \\
=\begin{pmatrix}
3197 & -1266 \\
7385 & -2922
\end{pmatrix}
\end{array}
$$
N8
$$
\begin{array}\
[[A,B],C]+[[B,C],A]+[[C,A],B] \\
=[AB-BA,C]+[BC-CB,A]+[CA-AC,B] \\
=(AB-BA)C-C(AB-BA)+(BC-CB)A-A(BC-CB)\\+(CA-AC)B+B(CA-AC) \\
=ABC-BAC-CAB+CBA+BCA-CBA\\-ABC+ACB+CAB-ACB-BCA+BAC\text{(по дистрибутивности)} \\
= \mathbb{O}\blacksquare \text{(по коммутативности)}
\end{array}
$$
N9
$$
\begin{array}\
(A-B)(A+B)=(A-B)A+(A-B)B \\
=A^{2}-BA+AB-B^{2}\neq A^{2}-B^{2} \\ \\
\text{Любые некоммутирующие матрицы, например:} \\
A=\begin{pmatrix}
1 & 3 \\
5 & 7
\end{pmatrix};\;B=\begin{pmatrix}
2 & 4 \\
6 & 8
\end{pmatrix}
\end{array}
$$
N10
$$
\begin{array}\
\text{Заметим, что:}\;[XE_{ij}]_{kl}=\left[
\begin{array}\
[X]_{ki}, j=l \\
0, j\neq l
\end{array}
\right. \\
\text{Тогда:}\;[E_{ij}E_{kl}]_{pr}=\left[
\begin{array}\
[E_{ij}]_{pk},l=r \\
0, l\neq r
\end{array}
\right. \\
=\left[
\begin{array}\
\left[
\begin{array}\
1, i=p \wedge l=r \\
0, i\neq p \vee l\neq r
\end{array}
\right.\;, j=k \\
0, j\neq k
\end{array}
\right. \\
=\left[
\begin{array}\
1, (i=p \wedge l=r) \wedge j \neq k \\
0, (i\neq p \vee l\neq r)\vee j \neq k
\end{array}
\right. \\ \\
\text{По опр. матричной единицы:}\;E_{ij}E_{kl}=\left[
\begin{array}\
E_{il}, j=k \\
0, j\neq k
\end{array}\;\;\blacksquare
\right.
\end{array}
$$
N11 
$$
\begin{array}\
i=4;\;j=2;\;A=\begin{pmatrix}
1  & 2 & 3 \\
4 & 5 & 6  \\
-1 & -2 & -3 \\
7 & 8 & 9
\end{pmatrix} \\ \\
(E+10E_{ij})A= \\
(\begin{pmatrix}
1 & 0 & 0 & 0 \\
0 & 1 & 0 & 0 \\
0 & 0 & 1 & 0 \\
0 & 0 & 0 & 1
\end{pmatrix}+\begin{pmatrix}
0 & 0 & 0 & 0 \\
0 & 0 & 0 & 0 \\
0 & 0 & 0 & 0 \\
0 & 0 & 10 & 0
\end{pmatrix})\cdot\begin{pmatrix}
1  & 2 & 3 \\
4 & 5 & 6  \\
-1 & -2 & -3 \\
7 & 8 & 9
\end{pmatrix} \\
=\begin{pmatrix}
1 & 0 & 0 & 0 \\
0 & 1 & 0 & 0 \\
0 & 0 & 1 & 0 \\
0 & 0 & 10 & 1
\end{pmatrix}\cdot \begin{pmatrix}
1  & 2 & 3 \\
4 & 5 & 6  \\
-1 & -2 & -3 \\
7 & 8 & 9
\end{pmatrix} \\
=\begin{pmatrix}
1 & 2 & 3 \\
4 & 5 & 6 \\
-1 & -2 & -3 \\
47 & 58 & 69
\end{pmatrix}
\end{array}
$$
$$
\begin{array}\
(E+\lambda E_{ij})A=EA+\lambda E_{ij}A=A+\lambda EijA \\
\text{К i-той строке A прибавляется }\lambda\text{ j-тых строк}
\end{array}
$$
N12
$$
\begin{array}\
[E_{ii}A]_{kl}=\left[
\begin{array}\
[A]_{il}, i=k \\
0, i\neq k
\end{array}
\right.;\; \\
[AE_{ii}]_{kl}=\left[
\begin{array}\
[A]_{ki},i=l \\
0, i\neq l
\end{array}
\right. \\
 \\
E_{ii}A=A_{ii} \Rightarrow [E_{ii}A]_{kl} = [AE_{ii}]_{kl} = \left[
\begin{array}\
[A]_{il}=[A]_{ki}, i=k=l \\
0, i\neq k \neq l
\end{array}
\right.  \\
[AE_{ii}]_{kl}= \left[
\begin{array}\
\left[
\begin{array}\
[A]_{kl}, k=l \\
0, k \neq l
\end{array}
\right. , i=l \\
0, i \neq l
\end{array}
\right. = \left[
\begin{array}\
[A]_{kl},i=l \\
0, i\neq l
\end{array}
\right. \text{  (По опр. матр. ед.)} \\
\Rightarrow [A]_{kl}=\left[
\begin{array}\
[A]_{kl}, k=l \\
0, k \neq l
\end{array}
\right.\;\;\; \blacksquare
\end{array}
$$
